Now we have obtain a contradiction for the other case. Suppose that $y^6 \equiv x_2^3 \equiv 1 \pmod 4 $, which implies that $y\equiv x_2 \equiv  1 \pmod 2$. Lets go further and assume that we may write $2^\alpha t = y^6 -1 $ and $2^\beta s = x_2^6 -1$ where $(t, 2) = (s, 2 ) = 1$ and $\alpha, \beta \geq 2$. Moreover, $x_2^6 + 4 x_1 ^6 =  y^6$ if and only if $x_2^6 + 4 x_1 ^6  - 1 =  y^6 -1$ and thus $4 x_1^6 + 2^{\alpha } s = 2^{\beta}t $, which implies that $x_2^6 \equiv 0 \pmod 2$ so $x_2 \equiv 0 \pmod 2$ and we can assume further $x_1 ^6= 2^c N$ for some $c \geq 1$ with $(2,N) = 1$. Thus we're focused on the equation $2^\alpha s + 2^c N = 2^\beta t$. We now have several cases to go through. We obviously cannot have that $\alpha = c = \beta$ and also if all of them are disistinct we have a contradiction. So, we consider overlapping values. If $\alpha = c$ and $\alpha > \beta$, then $2^{\alpha - \beta }s + 2^{c-\beta} N = t$, so the parities don't align. Now for , if $\alpha = c$ and $c < \beta$, then $ s + N = 2^{c - \beta} t$â€”the parity aligns here, however, we have that $\beta \geq 2$ so $s + N \equiv 0 \pmod 4$. But $2^c N + 2^\beta t + 2^s \alpha  = 2^c (N+s) + 2^\beta t = x_1^6 + x_2^6 + y^6 -2 \equiv 0 \pmod 4$, and as $y \equiv x_2 \equiv 1 \pmod 4$, then $(x_1^3)^2 +(x_2)^3$ 